instantiation lemma relocation, misc refactoring

theories/iris/iris_instantiation.v
@@ -5,178 +5,13 @@ From iris.base_logic Require Export gen_heap ghost_map proph_map.
 From iris.base_logic.lib Require Export fancy_updates.
 (* From iris.bi Require Export weakestpre. *)
 Require Export iris_locations iris_properties iris_rules_resources iris_wp_def stdpp_aux iris.
-Require Export datatypes host operations properties opsem instantiation.
+Require Export datatypes host operations properties opsem instantiation instantiation_properties.
 (* We need a few helper lemmas from preservation. *)
 Require Export type_preservation.
 
 Close Scope byte.
 
-Section module_typing_det.
-
-Lemma module_typing_det_import_aux m it1 et1 it2 et2:
-  module_typing m it1 et1 ->
-  module_typing m it2 et2 ->
-  it1 = it2.
-Proof.
-  move => Hmt1 Hmt2.
-  unfold module_typing in Hmt1, Hmt2.
-  destruct m.
-  destruct Hmt1 as [fts1 [gts1 [Hmft1 [Hmtt1 [Hmmt1 [Hmgt1 [Hmet1 [Hmdt1 [Hmst1 [Hmimt1 Hmext1]]]]]]]]]].
-  destruct Hmt2 as [fts2 [gts2 [Hmft2 [Hmtt2 [Hmmt2 [Hmgt2 [Hmet2 [Hmdt2 [Hmst2 [Hmimt2 Hmext2]]]]]]]]]].
-  
-  clear - Hmimt1 Hmimt2.
-  apply list_eq.
-  move => i.
-  rewrite -> Forall2_lookup in Hmimt1.
-  specialize (Hmimt1 i).
-  rewrite -> Forall2_lookup in Hmimt2.
-  specialize (Hmimt2 i).    
-  destruct (it1 !! i) eqn:Hitl1; destruct (it2 !! i) eqn:Hitl2; inversion Hmimt1; inversion Hmimt2; subst => //=.
-  - rewrite <- H in H2.
-    inversion H2; subst; clear H2.
-    destruct x; simpl in *.
-    unfold module_import_typing in *.
-    destruct imp_desc; simpl in *; destruct e; destruct e0 => //.
-    { (* func *)
-      move/andP in H1; destruct H1.
-      move/andP in H4; destruct H4.
-      destruct (nth_error mod_types n) => //.
-      move/eqP in H1.
-      move/eqP in H3.
-      by subst.
-    }
-    { (* table *)
-      move/andP in H1; destruct H1.
-      move/andP in H4; destruct H4.
-      move/eqP in H0.
-      move/eqP in H2.
-      by subst.
-    }
-    { (* memory *)
-      move/andP in H1; destruct H1.
-      move/andP in H4; destruct H4.
-      move/eqP in H0.
-      move/eqP in H2.
-      by subst.
-    }
-    { (* global *)
-      move/eqP in H1.
-      move/eqP in H4.
-      by subst.
-    }
-  - by rewrite <- H in H3.
-  - by rewrite <- H in H0.
-Qed.
-
-
-Lemma module_typing_det m it1 et1 it2 et2:
-  module_typing m it1 et1 ->
-  module_typing m it2 et2 ->
-  (it1, et1) = (it2, et2).
-Proof.
-  move => Hmt1 Hmt2.
-  specialize (module_typing_det_import_aux _ _ _ _ _ Hmt1 Hmt2) as ->.
-  unfold module_typing in Hmt1, Hmt2.
-  destruct m.
-  destruct Hmt1 as [fts1 [gts1 [Hmft1 [Hmtt1 [Hmmt1 [Hmgt1 [Hmet1 [Hmdt1 [Hmst1 [Hmimt1 Hmext1]]]]]]]]]].
-  destruct Hmt2 as [fts2 [gts2 [Hmft2 [Hmtt2 [Hmmt2 [Hmgt2 [Hmet2 [Hmdt2 [Hmst2 [Hmimt2 Hmext2]]]]]]]]]].
-
-  (* Function types *)
-  assert (fts1 = fts2) as Heqfts.
-  { clear - Hmft1 Hmft2.
-    apply list_eq.
-    move => i.
-    rewrite -> Forall2_lookup in Hmft1.
-    specialize (Hmft1 i).
-    rewrite -> Forall2_lookup in Hmft2.
-    specialize (Hmft2 i).
-    destruct (mod_funcs !! i) eqn: Hfli; inversion Hmft1; inversion Hmft2; subst => //=.
-    destruct m, modfunc_type, y, y0; simpl in *.
-    destruct H1 as [_ [Heqtf1 _]].
-    destruct H4 as [_ [Heqtf2 _]].
-    move/eqP in Heqtf1.
-    move/eqP in Heqtf2.
-    rewrite Heqtf1 in Heqtf2.
-    by rewrite Heqtf2.
-  }
-  subst.
-
-  (* Global types *)
-  assert (gts1 = gts2) as Heqgts.
-  { clear - Hmgt1 Hmgt2.
-    apply list_eq.
-    move => i.
-    rewrite -> Forall2_lookup in Hmgt1.
-    specialize (Hmgt1 i).
-    rewrite -> Forall2_lookup in Hmgt2.
-    specialize (Hmgt2 i).
-    destruct (mod_globals !! i) eqn: Hgli; inversion Hmgt1; inversion Hmgt2; subst => //=.
-    destruct m, modglob_type, y, y0; simpl in *.
-    destruct H1 as [_ [Heqgt1 _]].
-    destruct H4 as [_ [Heqgt2 _]].
-    inversion Heqgt1.
-    inversion Heqgt2.
-    by subst.
-  }
-  subst.
-  
-  f_equal.
-  clear - Hmext1 Hmext2.
-  apply list_eq.
-  move => i.
-  rewrite -> Forall2_lookup in Hmext1.
-  specialize (Hmext1 i).
-  rewrite -> Forall2_lookup in Hmext2.
-  specialize (Hmext2 i).    
-  destruct (et1 !! i) eqn:Hetl1; destruct (et2 !! i) eqn:Hetl2; inversion Hmext1; inversion Hmext2; subst => //=.
-  - rewrite <- H in H2.
-    inversion H2; subst; clear H2.
-    destruct x; simpl in *.
-    unfold module_export_typing in *.
-    destruct modexp_desc; [destruct f | destruct t | destruct m | destruct g]; simpl in *; destruct e; destruct e0 => //=.
-    { (* func *)
-      move/andP in H1; destruct H1.
-      move/andP in H4; destruct H4.
-      destruct (nth_error _ n) => //.
-      move/eqP in H1.
-      move/eqP in H3.
-      by subst.
-    }
-    { (* table *)
-      move/andP in H1; destruct H1.
-      move/andP in H4; destruct H4.
-      destruct (nth_error _ n) => //.
-      move/eqP in H1.
-      move/eqP in H3.
-      by subst.
-    }
-    { (* memory *)
-      move/andP in H1; destruct H1.
-      move/andP in H4; destruct H4.
-      destruct (nth_error _ n) => //.
-      move/eqP in H1.
-      move/eqP in H3.
-      by subst.
-    }
-    { (* global *)
-      move/andP in H1; destruct H1.
-      move/andP in H4; destruct H4.
-      destruct (nth_error _ n) => //.
-      move/eqP in H1.
-      move/eqP in H3.
-      by subst.
-    }
-  - by rewrite <- H in H3.
-  - by rewrite <- H in H0.
-Qed.    
-  
-End module_typing_det.
-
-
 Section Iris_instantiation.
-
-
-
 
 Definition assert_const1 (es: expr) : option value :=
   match es with
@@ -243,29 +78,6 @@ Definition module_data_bound_check_gmap (wms: gmap N memory) (imp_descs: list mo
 
 Context `{!wasmG Σ}.
 
-Definition ext_func_addrs := (map (fun x => match x with | Mk_funcidx i => i end)) ∘ ext_funcs.
-Definition ext_tab_addrs := (map (fun x => match x with | Mk_tableidx i => i end)) ∘ ext_tabs.
-Definition ext_mem_addrs := (map (fun x => match x with | Mk_memidx i => i end)) ∘ ext_mems.
-Definition ext_glob_addrs := (map (fun x => match x with | Mk_globalidx i => i end)) ∘ ext_globs.
-
-(* Getting the count of each type of imports from a module. This is to calculate the correct shift for indices of the exports in the Wasm store later.*)
-Definition get_import_func_count (m: module) := length (pmap (fun x => match x.(imp_desc) with
-                                                                   | ID_func id => Some id
-                                                                   | _ => None
-                                                                    end) m.(mod_imports)).
-
-Definition get_import_table_count (m: module) := length (pmap (fun x => match x.(imp_desc) with
-                                                                   | ID_table id => Some id
-                                                                   | _ => None
-                                                                    end) m.(mod_imports)).
-Definition get_import_mem_count (m: module) := length (pmap (fun x => match x.(imp_desc) with
-                                                                   | ID_mem id => Some id
-                                                                   | _ => None
-                                                                    end) m.(mod_imports)).
-Definition get_import_global_count (m: module) := length (pmap (fun x => match x.(imp_desc) with
-                                                                   | ID_global id => Some id
-                                                                   | _ => None
-                                                                    end) m.(mod_imports)).
 
 Definition import_resources_wasm_domcheck (v_imps: list module_export) (wfs: gmap N function_closure) (wts: gmap N tableinst) (wms: gmap N memory) (wgs: gmap N global) : iProp Σ :=
   ⌜ dom (gset N) wfs ≡ list_to_set (fmap N.of_nat (ext_func_addrs (fmap modexp_desc v_imps))) /\
@@ -371,47 +183,6 @@ Admitted.
  *)
 
 Definition exp_default := MED_func (Mk_funcidx 0).
-
-Lemma ext_tabs_lookup_exist (modexps: list module_export_desc) n tn:
-  (ext_tabs modexps) !! n = Some tn ->
-  exists k, modexps !! k = Some (MED_table tn).
-Proof.
-  move: n tn.
-  induction modexps; move => n tn Hexttablookup => //=.
-  simpl in Hexttablookup.
-  destruct a => //. 
-  2: { simpl in *.
-       destruct n; simpl in *; first by inversion Hexttablookup; subst; exists 0.
-       apply IHmodexps in Hexttablookup.
-       destruct Hexttablookup as [k ?].
-       by exists (S k).
-  }
-  all: simpl in *. 
-  all: apply IHmodexps in Hexttablookup.
-  all: destruct Hexttablookup as [k ?].
-  all: by exists (S k).
-Qed.
-
-Lemma ext_mems_lookup_exist (modexps: list module_export_desc) n mn:
-  (ext_mems modexps) !! n = Some mn ->
-  exists k, modexps !! k = Some (MED_mem mn).
-Proof.
-  move: n mn.
-  induction modexps; move => n mn Hextmemlookup => //=.
-  simpl in Hextmemlookup.
-  destruct a => //. 
-  3: { simpl in *.
-       destruct n; simpl in *; first try by inversion Hextmemlookup; subst; exists 0.
-       apply IHmodexps in Hextmemlookup.
-       destruct Hextmemlookup as [k ?].
-       by exists (S k).
-  }
-  all: simpl in *. 
-  all: apply IHmodexps in Hextmemlookup.
-  all: destruct Hextmemlookup as [k ?].
-  all: by exists (S k).
-Qed.
-
 
 Lemma import_resources_wasm_lookup v_imps t_imps wfs wts wms wgs ws:
   ⊢ gen_heap_interp (gmap_of_list (s_funcs ws)) -∗
@@ -657,240 +428,6 @@ Proof.
   by rewrite Hmdata.
 Qed.
 
-Definition gen_index offset len : list nat :=
-  imap (fun i x => i+offset+x) (repeat 0 len).
-
-Lemma gen_index_lookup offset len k:
-  k < len ->
-  (gen_index offset len) !! k = Some (offset + k).
-Proof.
-  move => Hlen.
-  unfold gen_index.
-  rewrite list_lookup_imap => /=.
-  eapply repeat_lookup with (x := 0) in Hlen.
-  rewrite Hlen.
-  simpl.
-  f_equal.
-  by lias.
-Qed.
-
-Lemma gen_index_extend offset len:
-  gen_index offset (len+1) = gen_index offset len ++ [::offset+len].
-Proof.
-  unfold gen_index.
-  rewrite repeat_app => /=.
-  induction len => //=.
-  f_equal => //.
-  do 2 rewrite - fmap_imap.
-  rewrite IHlen.
-  rewrite fmap_app => /=.
-  repeat f_equal.
-  by lias.
-Qed.
-
-Lemma combine_app {T1 T2: Type} (l1 l3: list T1) (l2 l4: list T2):
-  length l1 = length l2 ->
-  combine (l1 ++ l3) (l2 ++ l4) = combine l1 l2 ++ combine l3 l4.
-Proof.
-  generalize dependent l2.
-  generalize dependent l3.
-  generalize dependent l4.
-  induction l1; move => l4 l3 l2 Hlen => /=; first by destruct l2 => //.
-  - destruct l2 => //=.
-    simpl in Hlen.
-    inversion Hlen; subst; clear Hlen.
-    f_equal.
-    by apply IHl1.
-Qed.
-
-Definition gen_func_instance mf inst : function_closure :=
-  let ft := nth match modfunc_type mf with
-                | Mk_typeidx n => n
-                end (inst_types inst) (Tf [] []) in
-  FC_func_native inst ft (modfunc_locals mf) (modfunc_body mf).
-                
-
-(* This is an actual interesting proof, technically *)
-(* TODO: see if it's possible to refactor the 4 proofs into one *)
-Lemma alloc_func_gen_index modfuncs ws inst ws' l:
-  alloc_funcs ws modfuncs inst = (ws', l) ->
-  map (fun x => match x with | Mk_funcidx i => i end) l = gen_index (length (s_funcs ws)) (length modfuncs) /\
-  ws'.(s_funcs) = ws.(s_funcs) ++ fmap (fun mf => gen_func_instance mf inst) modfuncs /\
- (* length ws'.(s_funcs) = length ws.(s_funcs) + length modfuncs /\*)
-  ws.(s_tables) = ws'.(s_tables) /\
-  ws.(s_mems) = ws'.(s_mems) /\
-  ws.(s_globals) = ws'.(s_globals).
-Proof.
-  unfold alloc_funcs, alloc_Xs.
-  generalize dependent l.
-  generalize dependent ws'.
-  generalize dependent ws.
-  induction modfuncs using List.rev_ind; move => ws ws' l Hallocfuncs.
-  - inversion Hallocfuncs; subst; clear Hallocfuncs.
-    simpl.
-    repeat split => //.
-    by rewrite app_nil_r.
-  - rewrite fold_left_app in Hallocfuncs.
-    remember (fold_left _ modfuncs (ws,[])) as fold_res.
-    simpl in Hallocfuncs.
-    destruct fold_res as [ws0 l0].
-    symmetry in Heqfold_res.
-    unfold add_func in Hallocfuncs.
-    inversion Hallocfuncs; subst; clear Hallocfuncs.
-    rewrite map_app app_length /=.
-    rewrite gen_index_extend.
-    specialize (IHmodfuncs ws ws0 (rev l0)).
-    destruct IHmodfuncs as [? [? [? [? ?]]]]; first by rewrite Heqfold_res.
-    repeat split => //; try by eapply IHmodfuncs; rewrite Heqfold_res.
-    + rewrite H.
-      rewrite H0.
-      by rewrite app_length map_length.
-    + rewrite H0.
-      rewrite - app_assoc.
-      f_equal.
-      by rewrite -> list_fmap_app.
-Qed.
-
-Lemma alloc_tab_gen_index modtabtypes ws ws' l:
-  alloc_tabs ws modtabtypes = (ws', l) ->
-  map (fun x => match x with | Mk_tableidx i => i end) l = gen_index (length (s_tables ws)) (length modtabtypes) /\
-  ws'.(s_tables) = ws.(s_tables) ++ fmap (fun '{| tt_limits := {| lim_min := min; lim_max := maxo |} |} => {| table_data := repeat None (ssrnat.nat_of_bin min); table_max_opt := maxo |}) modtabtypes /\
-  ws.(s_funcs) = ws'.(s_funcs) /\
-  ws.(s_mems) = ws'.(s_mems) /\
-  ws.(s_globals) = ws'.(s_globals).
-Proof.
-  unfold alloc_tabs, alloc_Xs.
-  generalize dependent l.
-  generalize dependent ws'.
-  generalize dependent ws.
-  induction modtabtypes using List.rev_ind; move => ws ws' l Halloc.
-  - inversion Halloc; subst; clear Halloc.
-    repeat split => //.
-    simpl.
-    by rewrite app_nil_r.
-  - rewrite fold_left_app in Halloc.
-    remember (fold_left _ modtabtypes (ws,[])) as fold_res.
-    simpl in Halloc.
-    destruct fold_res as [ws0 l0].
-    symmetry in Heqfold_res.
-    unfold alloc_tab, add_table in Halloc.
-    destruct x => /=.
-    destruct tt_limits => /=.
-    specialize (IHmodtabtypes ws ws0 (rev l0)).
-    rewrite Heqfold_res in IHmodtabtypes.
-    inversion Halloc; subst; clear Halloc.
-    simpl in *.
-    rewrite map_app app_length /=.
-    rewrite gen_index_extend.
-    destruct IHmodtabtypes as [? [? [? [? ?]]]] => //.
-    repeat split => //.
-    + rewrite H.
-      rewrite H0.
-      by rewrite app_length map_length.
-    + rewrite H0.
-      rewrite - app_assoc.
-      f_equal.
-      by rewrite -> list_fmap_app => /=.
-Qed.
-
-Lemma alloc_mem_gen_index modmemtypes ws ws' l:
-  alloc_mems ws modmemtypes = (ws', l) ->
-  map (fun x => match x with | Mk_memidx i => i end) l = gen_index (length (s_mems ws)) (length modmemtypes) /\
-  ws'.(s_mems) = ws.(s_mems) ++ fmap (fun '{| lim_min := min; lim_max := maxo |} => {| mem_data := mem_make #00%byte (page_size * min)%N; mem_max_opt := maxo |}) modmemtypes /\
-  ws.(s_funcs) = ws'.(s_funcs) /\
-  ws.(s_tables) = ws'.(s_tables) /\
-  ws.(s_globals) = ws'.(s_globals).
-Proof.
-  unfold alloc_mems, alloc_Xs.
-  generalize dependent l.
-  generalize dependent ws'.
-  generalize dependent ws.
-  induction modmemtypes using List.rev_ind; move => ws ws' l Halloc.
-  - inversion Halloc; subst; clear Halloc.
-    repeat split => //=.
-    by rewrite app_nil_r.
-  - rewrite fold_left_app in Halloc.
-    remember (fold_left _ modmemtypes (ws,[])) as fold_res.
-    simpl in Halloc.
-    destruct fold_res as [ws0 l0].
-    symmetry in Heqfold_res.
-    unfold alloc_mem, add_mem in Halloc.
-    destruct x => /=.
-    specialize (IHmodmemtypes ws ws0 (rev l0)).
-    rewrite Heqfold_res in IHmodmemtypes.
-    inversion Halloc; subst; clear Halloc.
-    simpl in *.
-    rewrite map_app app_length /=.
-    rewrite gen_index_extend.
-    destruct IHmodmemtypes as [? [? [? [? ?]]]] => //.
-    repeat split => //.
-    + rewrite H.
-      rewrite H0.
-      by rewrite app_length fmap_length.
-    + rewrite H0.
-      rewrite - app_assoc.
-      f_equal.
-      by rewrite -> list_fmap_app => /=.
-Qed.
-
-Lemma alloc_glob_gen_index modglobs ws g_inits ws' l:
-  length g_inits = length modglobs ->
-  alloc_globs ws modglobs g_inits = (ws', l) ->
-  map (fun x => match x with | Mk_globalidx i => i end) l = gen_index (length (s_globals ws)) (length modglobs) /\
-  ws'.(s_globals) = ws.(s_globals) ++ fmap (fun '({| modglob_type := gt; modglob_init := ge |}, v) => {| g_mut := gt.(tg_mut); g_val := v |} ) (combine modglobs g_inits) /\
- (* length ws'.(s_globals) = length ws.(s_globals) + length modglobs /\*)
-  ws.(s_funcs) = ws'.(s_funcs) /\
-  ws.(s_tables) = ws'.(s_tables) /\
-  ws.(s_mems) = ws'.(s_mems).
-Proof.
-  unfold alloc_globs, alloc_Xs.
-  generalize dependent l.
-  generalize dependent ws'.
-  generalize dependent ws.
-  generalize dependent g_inits.
-  induction modglobs using List.rev_ind; move => g_inits ws ws' l Hlen Halloc.
-  - inversion Halloc; subst; clear Halloc.
-    repeat split => //=.
-    by rewrite app_nil_r.
-  - destruct g_inits using List.rev_ind; first by destruct modglobs => /=.
-    repeat rewrite app_length in Hlen; simpl in Hlen.
-    repeat rewrite - cat_app in Halloc.
-    rewrite combine_app in Halloc; last by lias.
-    simpl in Halloc.
-    rewrite fold_left_app in Halloc.
-    lazymatch goal with
-    | _: context C [fold_left ?f (combine modglobs g_inits) (ws, [])] |- _ =>
-      remember (fold_left f (combine modglobs g_inits) (ws, [])) as fold_res
-    end.
-    (* rewrite - Heqfold_res in Halloc. *)
-    destruct fold_res as [ws0 l0].
-    symmetry in Heqfold_res.
-    unfold alloc_glob, add_glob in Halloc.
-    simpl in Halloc.
-    inversion Halloc; subst; clear Halloc.
-    rewrite map_app app_length /=.
-    rewrite gen_index_extend.
-    specialize (IHmodglobs g_inits ws ws0 (rev l0)).
-    destruct IHmodglobs as [? [? [? [? ?]]]] => //.
-    + by lias.
-    + by rewrite Heqfold_res.
-    repeat split => //.
-    + rewrite H.
-      rewrite H0.
-      rewrite app_length fmap_length combine_length.
-      repeat f_equal.
-      by lias.
-    + rewrite H0.
-      rewrite - app_assoc.
-      f_equal.
-      rewrite combine_app => /=.
-      rewrite -> list_fmap_app => /=.
-      repeat f_equal.
-      destruct x => //.
-      by lias.
-Qed.
-
-
 Definition module_glob_init_value (modglobs: list module_glob): option (list value) :=
   those (fmap (assert_const1 ∘ modglob_init) modglobs).
 
@@ -974,15 +511,6 @@ Proof.
   rewrite take_length drop_length.
   by lias.
 Qed.
-
-(*
-Lemma fold_left_preserve {A B: Type} (P: A -> Prop) (f: A -> B -> A) (l: list B) (acc: A):
-  P acc ->
-  (forall (x:A) (act: B), P x -> P (f x act)) ->
-  P (fold_left f l acc).
-Proof.
-Admitted.
-*)
 
 (* Each of these is guaranteed to be a some due to validation. *)
 Definition lookup_funcaddr (inst: instance) (me_init: list funcidx) : list funcelem :=
@@ -1171,25 +699,6 @@ Definition module_restrictions (m: module) : Prop :=
   (exists (vi32s: list i32), fmap modelem_offset m.(mod_elem) = fmap (fun v => [BI_const (VAL_int32 v)]) vi32s) /\
   (exists (vi32s: list i32), fmap moddata_offset m.(mod_data) = fmap (fun v => [BI_const (VAL_int32 v)]) vi32s).
 
-Lemma fmap_fmap_lookup {T1 T2 T: Type} (f1: T1 -> T) (f2: T2 -> T) (l1: list T1) (l2: list T2):
-  fmap f1 l1 = fmap f2 l2 ->
-  forall i, fmap f1 (l1 !! i) = fmap f2 (l2 !! i).
-Proof.
-  move => Heq i.
-  assert (length l1 = length l2) as Hlen.
-  { erewrite <- fmap_length with (f := f1).
-    rewrite Heq.
-    by rewrite fmap_length.
-  }
-  destruct (l1 !! i) eqn:Hl1; destruct (l2 !! i) eqn:Hl2 => //=.
-  - assert ((fmap f1 l1) !! i = (fmap f2 l2) !! i) as Heqi; first by rewrite Heq.
-    repeat rewrite list_lookup_fmap in Heqi.
-    rewrite Hl1 Hl2 in Heqi.
-    by simpl in Heqi.
-  - by apply lookup_lt_Some in Hl1; apply lookup_ge_None in Hl2; lias.
-  - by apply lookup_lt_Some in Hl2; apply lookup_ge_None in Hl1; lias.
-Qed.
-
 Lemma BI_const_assert_const1_i32 (es: list expr) (vs: list i32):
   es = fmap (fun v => [BI_const (VAL_int32 v)]) vs ->
   those (fmap assert_const1_i32 es) = Some vs.
@@ -1206,70 +715,6 @@ Proof.
     by [].
 Qed.
 
-Lemma all2_Forall2 {T1 T2: Type} r (l1: list T1) (l2: list T2):
-  all2 r l1 l2 <-> Forall2 r l1 l2.
-Proof.
-  move: l2.
-  elim: l1 => //=.
-  - move => l2; destruct l2 => //=.
-    split => //.
-    move => Hcontra.
-    by inversion Hcontra.
-  - move => e l1 IH l2.
-    destruct l2 => //=.
-    + split => //.
-      move => Hcontra.
-      by inversion Hcontra.
-    + split; move => H.
-      * move/andP in H.
-        destruct H.
-        constructor => //.
-        by apply IH.
-      * apply/andP.
-        inversion H; subst; clear H.
-        split => //.
-        by apply IH.
-Qed.
-
-Lemma map_fmap {T1 T2: Type} (f: T1 -> T2) (l: list T1):
-  map f l = fmap f l.
-Proof.
-  trivial.
-Qed.
-
-(* Ok, this is not built-in, but fair enough since it is across 3 libraries *)
-Lemma N_nat_bin n:
-  n = N.of_nat (ssrnat.nat_of_bin n).
-Proof.
-  destruct n => //=.
-  replace (ssrnat.nat_of_pos p) with (Pos.to_nat p); first by rewrite positive_nat_N.
-  induction p => //=.
-  - rewrite Pos2Nat.inj_xI.
-    f_equal.
-    rewrite IHp.
-    rewrite ssrnat.NatTrec.doubleE.
-    rewrite - ssrnat.mul2n.
-    by lias.
-  - rewrite Pos2Nat.inj_xO.
-    rewrite IHp.
-    rewrite ssrnat.NatTrec.doubleE.
-    rewrite - ssrnat.mul2n.
-    by lias.
-Qed.
-
-Lemma fold_left_preserve {A B: Type} (P: A -> Prop) (f: A -> B -> A) (l: list B) (acc: A) :
-  P acc ->
-  (forall (x:A) (act: B), P x -> P (f x act)) ->
-  P (fold_left f l acc).
-Proof.
-  rewrite -fold_left_rev_right.
-  revert acc.
-  induction l;simpl;auto.
-  intros acc Ha Hnext.
-  rewrite foldr_snoc /=. apply IHl =>//.
-  apply Hnext=>//.
-Qed.    
-  
 Lemma module_inst_build_tables_length m i :
   length (module_inst_build_tables m i) = length (mod_tables m).
 Proof.
@@ -1282,8 +727,6 @@ Proof.
     destruct (nth_error x (n - get_import_table_count m));auto.
     rewrite insert_length//. }
 Qed.
-
-
 
 Ltac forward H Hname :=
   lazymatch type of H with
@@ -1954,24 +1397,6 @@ Proof.
     iFrame.
 Admitted.
 
-Lemma init_tabs_preserve ws inst e_inits melem ws':
-  init_tabs ws inst e_inits melem = ws' ->
-  ws.(s_funcs) = ws'.(s_funcs) /\
-  ws.(s_mems) = ws'.(s_mems) /\
-  ws.(s_globals) = ws'.(s_globals).
-Proof.
-  move => Hinit.
-  unfold init_tabs in Hinit.
-  rewrite - Hinit.
-  apply fold_left_preserve => //.
-  move => x [n me] Heq.
-  destruct ws, x.
-  simpl in *.
-  destruct Heq as [-> [-> ->]].
-  unfold init_tab => /=.
-  by destruct (nth _ _) eqn:Hl => /=.
-Qed.
-  
 Lemma init_mems_state_update ws ws' inst d_inits m v_imps t_imps wfs wts wms wgs:
   let wms' := module_import_init_mems m inst wms in
   ⌜init_mems ws inst d_inits m.(mod_data) = ws'⌝ -∗
@@ -1998,62 +1423,6 @@ Lemma init_mems_state_update ws ws' inst d_inits m v_imps t_imps wfs wts wms wgs
   module_inst_resources_mem (module_inst_build_mems m inst) (drop (get_import_mem_count m) inst.(inst_memory))))%I.
 Proof.
 Admitted.
-
-Lemma init_mems_preserve ws inst d_inits mdata ws':
-  init_mems ws inst d_inits mdata = ws' ->
-  ws.(s_funcs) = ws'.(s_funcs) /\
-  ws.(s_tables) = ws'.(s_tables) /\
-  ws.(s_globals) = ws'.(s_globals).
-Proof.
-  move => Hinit.
-  unfold init_mems in Hinit.
-  rewrite - Hinit.
-  apply fold_left_preserve => //.
-  move => x [n md] Heq.
-  destruct ws, x.
-  simpl in *.
-  destruct Heq as [-> [-> ->]].
-  by unfold init_mem => /=.
-Qed.
-
-Lemma mod_imps_len_t m t_imps t_exps:
-  module_typing m t_imps t_exps ->
-  get_import_func_count m = length (ext_t_funcs t_imps) /\
-  get_import_table_count m = length (ext_t_tabs t_imps) /\
-  get_import_mem_count m = length (ext_t_mems t_imps) /\
-  get_import_global_count m = length (ext_t_globs t_imps).
-Proof.
-  unfold get_import_func_count, get_import_table_count, get_import_mem_count, get_import_global_count.
-  unfold module_typing.
-  move => Hmt.
-  destruct m.
-  destruct Hmt as [fts [gts [? [? [? [? [? [? [? [Himptype ?]]]]]]]]]].
-  simpl in *.
-  clear - mod_imports Himptype.
-  move : Himptype.
-  move : t_imps fts gts.
-  induction mod_imports; move => t_imps fts gts Himptype => //=.
-  - apply Forall2_nil_inv_l in Himptype as ->.
-    by simpl.
-  - destruct t_imps; first by apply Forall2_nil_inv_r in Himptype.
-    simpl in *.
-    inversion Himptype; subst; clear Himptype.
-    unfold module_import_typing in H2.
-    destruct a, imp_desc => /=; simpl in H2; destruct e => //.
-    all:
-      try by (move/andP in H2;
-      destruct H2 as [Hlen Hnth];
-      move/eqP in Hnth; subst;
-      simpl;
-      apply IHmod_imports in H4 as [? [? [? ?]]] => //;
-      repeat split => //;
-      f_equal).
-    move/eqP in H2; subst.
-    simpl.
-    apply IHmod_imports in H4 as [? [? [? ?]]] => //.
-    repeat split => //.
-    by f_equal.
-Qed.
 
 Lemma module_inst_build_tables_nil m inst:
   m.(mod_tables) = [] ->
