theories/instantiation_properties.v
@@ -1,0 +1,578 @@
+From mathcomp Require Import ssreflect eqtype seq ssrbool ssrfun.
+Require Export datatypes host operations properties opsem instantiation.
+From stdpp Require Import list fin_maps gmap.
+Require Export stdpp_aux.
+(* We need a few helper lemmas from preservation. *)
+Require Export type_preservation.
+
+Section module_typing_det.
+
+Lemma module_typing_det_import_aux m it1 et1 it2 et2:
+  module_typing m it1 et1 ->
+  module_typing m it2 et2 ->
+  it1 = it2.
+Proof.
+  move => Hmt1 Hmt2.
+  unfold module_typing in Hmt1, Hmt2.
+  destruct m.
+  destruct Hmt1 as [fts1 [gts1 [Hmft1 [Hmtt1 [Hmmt1 [Hmgt1 [Hmet1 [Hmdt1 [Hmst1 [Hmimt1 Hmext1]]]]]]]]]].
+  destruct Hmt2 as [fts2 [gts2 [Hmft2 [Hmtt2 [Hmmt2 [Hmgt2 [Hmet2 [Hmdt2 [Hmst2 [Hmimt2 Hmext2]]]]]]]]]].
+  
+  clear - Hmimt1 Hmimt2.
+  apply list_eq.
+  move => i.
+  rewrite -> Forall2_lookup in Hmimt1.
+  specialize (Hmimt1 i).
+  rewrite -> Forall2_lookup in Hmimt2.
+  specialize (Hmimt2 i).    
+  destruct (it1 !! i) eqn:Hitl1; destruct (it2 !! i) eqn:Hitl2; inversion Hmimt1; inversion Hmimt2; subst => //=.
+  - rewrite <- H in H2.
+    inversion H2; subst; clear H2.
+    destruct x; simpl in *.
+    unfold module_import_typing in *.
+    destruct imp_desc; simpl in *; destruct e; destruct e0 => //.
+    { (* func *)
+      move/andP in H1; destruct H1.
+      move/andP in H4; destruct H4.
+      destruct (nth_error mod_types n) => //.
+      move/eqP in H1.
+      move/eqP in H3.
+      by subst.
+    }
+    { (* table *)
+      move/andP in H1; destruct H1.
+      move/andP in H4; destruct H4.
+      move/eqP in H0.
+      move/eqP in H2.
+      by subst.
+    }
+    { (* memory *)
+      move/andP in H1; destruct H1.
+      move/andP in H4; destruct H4.
+      move/eqP in H0.
+      move/eqP in H2.
+      by subst.
+    }
+    { (* global *)
+      move/eqP in H1.
+      move/eqP in H4.
+      by subst.
+    }
+  - by rewrite <- H in H3.
+  - by rewrite <- H in H0.
+Qed.
+
+
+Lemma module_typing_det m it1 et1 it2 et2:
+  module_typing m it1 et1 ->
+  module_typing m it2 et2 ->
+  (it1, et1) = (it2, et2).
+Proof.
+  move => Hmt1 Hmt2.
+  specialize (module_typing_det_import_aux _ _ _ _ _ Hmt1 Hmt2) as ->.
+  unfold module_typing in Hmt1, Hmt2.
+  destruct m.
+  destruct Hmt1 as [fts1 [gts1 [Hmft1 [Hmtt1 [Hmmt1 [Hmgt1 [Hmet1 [Hmdt1 [Hmst1 [Hmimt1 Hmext1]]]]]]]]]].
+  destruct Hmt2 as [fts2 [gts2 [Hmft2 [Hmtt2 [Hmmt2 [Hmgt2 [Hmet2 [Hmdt2 [Hmst2 [Hmimt2 Hmext2]]]]]]]]]].
+
+  (* Function types *)
+  assert (fts1 = fts2) as Heqfts.
+  { clear - Hmft1 Hmft2.
+    apply list_eq.
+    move => i.
+    rewrite -> Forall2_lookup in Hmft1.
+    specialize (Hmft1 i).
+    rewrite -> Forall2_lookup in Hmft2.
+    specialize (Hmft2 i).
+    destruct (mod_funcs !! i) eqn: Hfli; inversion Hmft1; inversion Hmft2; subst => //=.
+    destruct m, modfunc_type, y, y0; simpl in *.
+    destruct H1 as [_ [Heqtf1 _]].
+    destruct H4 as [_ [Heqtf2 _]].
+    move/eqP in Heqtf1.
+    move/eqP in Heqtf2.
+    rewrite Heqtf1 in Heqtf2.
+    by rewrite Heqtf2.
+  }
+  subst.
+
+  (* Global types *)
+  assert (gts1 = gts2) as Heqgts.
+  { clear - Hmgt1 Hmgt2.
+    apply list_eq.
+    move => i.
+    rewrite -> Forall2_lookup in Hmgt1.
+    specialize (Hmgt1 i).
+    rewrite -> Forall2_lookup in Hmgt2.
+    specialize (Hmgt2 i).
+    destruct (mod_globals !! i) eqn: Hgli; inversion Hmgt1; inversion Hmgt2; subst => //=.
+    destruct m, modglob_type, y, y0; simpl in *.
+    destruct H1 as [_ [Heqgt1 _]].
+    destruct H4 as [_ [Heqgt2 _]].
+    inversion Heqgt1.
+    inversion Heqgt2.
+    by subst.
+  }
+  subst.
+  
+  f_equal.
+  clear - Hmext1 Hmext2.
+  apply list_eq.
+  move => i.
+  rewrite -> Forall2_lookup in Hmext1.
+  specialize (Hmext1 i).
+  rewrite -> Forall2_lookup in Hmext2.
+  specialize (Hmext2 i).    
+  destruct (et1 !! i) eqn:Hetl1; destruct (et2 !! i) eqn:Hetl2; inversion Hmext1; inversion Hmext2; subst => //=.
+  - rewrite <- H in H2.
+    inversion H2; subst; clear H2.
+    destruct x; simpl in *.
+    unfold module_export_typing in *.
+    destruct modexp_desc; [destruct f | destruct t | destruct m | destruct g]; simpl in *; destruct e; destruct e0 => //=.
+    { (* func *)
+      move/andP in H1; destruct H1.
+      move/andP in H4; destruct H4.
+      destruct (nth_error _ n) => //.
+      move/eqP in H1.
+      move/eqP in H3.
+      by subst.
+    }
+    { (* table *)
+      move/andP in H1; destruct H1.
+      move/andP in H4; destruct H4.
+      destruct (nth_error _ n) => //.
+      move/eqP in H1.
+      move/eqP in H3.
+      by subst.
+    }
+    { (* memory *)
+      move/andP in H1; destruct H1.
+      move/andP in H4; destruct H4.
+      destruct (nth_error _ n) => //.
+      move/eqP in H1.
+      move/eqP in H3.
+      by subst.
+    }
+    { (* global *)
+      move/andP in H1; destruct H1.
+      move/andP in H4; destruct H4.
+      destruct (nth_error _ n) => //.
+      move/eqP in H1.
+      move/eqP in H3.
+      by subst.
+    }
+  - by rewrite <- H in H3.
+  - by rewrite <- H in H0.
+Qed.    
+  
+End module_typing_det.
+
+Lemma N_nat_bin n:
+  n = N.of_nat (ssrnat.nat_of_bin n).
+Proof.
+  destruct n => //=.
+  replace (ssrnat.nat_of_pos p) with (Pos.to_nat p); first by rewrite positive_nat_N.
+  induction p => //=.
+  - rewrite Pos2Nat.inj_xI.
+    f_equal.
+    rewrite IHp.
+    rewrite ssrnat.NatTrec.doubleE.
+    rewrite - ssrnat.mul2n.
+    by lias.
+  - rewrite Pos2Nat.inj_xO.
+    rewrite IHp.
+    rewrite ssrnat.NatTrec.doubleE.
+    rewrite - ssrnat.mul2n.
+    by lias.
+Qed.
+
+Lemma fold_left_preserve {A B: Type} (P: A -> Prop) (f: A -> B -> A) (l: list B) (acc: A) :
+  P acc ->
+  (forall (x:A) (act: B), P x -> P (f x act)) ->
+  P (fold_left f l acc).
+Proof.
+  rewrite -fold_left_rev_right.
+  revert acc.
+  induction l;simpl;auto.
+  intros acc Ha Hnext.
+  rewrite foldr_snoc /=. apply IHl =>//.
+  apply Hnext=>//.
+Qed.    
+
+Section Instantiation_properties.
+
+Definition assert_const1 (es: expr) : option value :=
+  match es with
+  | [:: BI_const v] => Some v
+  | _ => None
+  end.
+
+Definition assert_const1_i32 (es: expr) : option i32 :=
+  match es with
+  | [:: BI_const (VAL_int32 v)] => Some v
+  | _ => None
+  end.
+
+Definition assert_const1_i32_to_nat (es:expr) : nat :=
+  match assert_const1_i32 es with
+  | Some v => nat_of_int v
+  | _ => 0
+  end.
+
+Definition ext_func_addrs := (map (fun x => match x with | Mk_funcidx i => i end)) ∘ ext_funcs.
+Definition ext_tab_addrs := (map (fun x => match x with | Mk_tableidx i => i end)) ∘ ext_tabs.
+Definition ext_mem_addrs := (map (fun x => match x with | Mk_memidx i => i end)) ∘ ext_mems.
+Definition ext_glob_addrs := (map (fun x => match x with | Mk_globalidx i => i end)) ∘ ext_globs.
+
+(* Getting the count of each type of imports from a module. This is to calculate the correct shift for indices of the exports in the Wasm store later. *)
+Definition get_import_func_count (m: module) := length (pmap (fun x => match x.(imp_desc) with
+                                                                   | ID_func id => Some id
+                                                                   | _ => None
+                                                                    end) m.(mod_imports)).
+
+Definition get_import_table_count (m: module) := length (pmap (fun x => match x.(imp_desc) with
+                                                                   | ID_table id => Some id
+                                                                   | _ => None
+                                                                    end) m.(mod_imports)).
+Definition get_import_mem_count (m: module) := length (pmap (fun x => match x.(imp_desc) with
+                                                                   | ID_mem id => Some id
+                                                                   | _ => None
+                                                                    end) m.(mod_imports)).
+Definition get_import_global_count (m: module) := length (pmap (fun x => match x.(imp_desc) with
+                                                                   | ID_global id => Some id
+                                                                   | _ => None
+                                                                      end) m.(mod_imports)).
+
+Lemma ext_tabs_lookup_exist (modexps: list module_export_desc) n tn:
+  (ext_tabs modexps) !! n = Some tn ->
+  exists k, modexps !! k = Some (MED_table tn).
+Proof.
+  move: n tn.
+  induction modexps; move => n tn Hexttablookup => //=.
+  simpl in Hexttablookup.
+  destruct a => //. 
+  2: { simpl in *.
+       destruct n; simpl in *; first by inversion Hexttablookup; subst; exists 0.
+       apply IHmodexps in Hexttablookup.
+       destruct Hexttablookup as [k ?].
+       by exists (S k).
+  }
+  all: simpl in *. 
+  all: apply IHmodexps in Hexttablookup.
+  all: destruct Hexttablookup as [k ?].
+  all: by exists (S k).
+Qed.
+
+Lemma ext_mems_lookup_exist (modexps: list module_export_desc) n mn:
+  (ext_mems modexps) !! n = Some mn ->
+  exists k, modexps !! k = Some (MED_mem mn).
+Proof.
+  move: n mn.
+  induction modexps; move => n mn Hextmemlookup => //=.
+  simpl in Hextmemlookup.
+  destruct a => //. 
+  3: { simpl in *.
+       destruct n; simpl in *; first try by inversion Hextmemlookup; subst; exists 0.
+       apply IHmodexps in Hextmemlookup.
+       destruct Hextmemlookup as [k ?].
+       by exists (S k).
+  }
+  all: simpl in *. 
+  all: apply IHmodexps in Hextmemlookup.
+  all: destruct Hextmemlookup as [k ?].
+  all: by exists (S k).
+Qed.
+
+Definition gen_index offset len : list nat :=
+  imap (fun i x => i+offset+x) (repeat 0 len).
+
+Lemma gen_index_lookup offset len k:
+  k < len ->
+  (gen_index offset len) !! k = Some (offset + k).
+Proof.
+  move => Hlen.
+  unfold gen_index.
+  rewrite list_lookup_imap => /=.
+  eapply repeat_lookup with (x := 0) in Hlen.
+  rewrite Hlen.
+  simpl.
+  f_equal.
+  by lias.
+Qed.
+
+Lemma gen_index_extend offset len:
+  gen_index offset (len+1) = gen_index offset len ++ [::offset+len].
+Proof.
+  unfold gen_index.
+  rewrite repeat_app => /=.
+  induction len => //=.
+  f_equal => //.
+  do 2 rewrite - fmap_imap.
+  rewrite IHlen.
+  rewrite fmap_app => /=.
+  repeat f_equal.
+  by lias.
+Qed.
+
+Definition gen_func_instance mf inst : function_closure :=
+  let ft := nth match modfunc_type mf with
+                | Mk_typeidx n => n
+                end (inst_types inst) (Tf [] []) in
+  FC_func_native inst ft (modfunc_locals mf) (modfunc_body mf).
+                
+
+(* This is an actual interesting proof, technically *)
+(* TODO: see if it's possible to refactor the 4 proofs into one *)
+Lemma alloc_func_gen_index modfuncs ws inst ws' l:
+  alloc_funcs ws modfuncs inst = (ws', l) ->
+  map (fun x => match x with | Mk_funcidx i => i end) l = gen_index (length (s_funcs ws)) (length modfuncs) /\
+  ws'.(s_funcs) = ws.(s_funcs) ++ fmap (fun mf => gen_func_instance mf inst) modfuncs /\
+ (* length ws'.(s_funcs) = length ws.(s_funcs) + length modfuncs /\*)
+  ws.(s_tables) = ws'.(s_tables) /\
+  ws.(s_mems) = ws'.(s_mems) /\
+  ws.(s_globals) = ws'.(s_globals).
+Proof.
+  unfold alloc_funcs, alloc_Xs.
+  generalize dependent l.
+  generalize dependent ws'.
+  generalize dependent ws.
+  induction modfuncs using List.rev_ind; move => ws ws' l Hallocfuncs.
+  - inversion Hallocfuncs; subst; clear Hallocfuncs.
+    simpl.
+    repeat split => //.
+    by rewrite app_nil_r.
+  - rewrite fold_left_app in Hallocfuncs.
+    remember (fold_left _ modfuncs (ws,[])) as fold_res.
+    simpl in Hallocfuncs.
+    destruct fold_res as [ws0 l0].
+    symmetry in Heqfold_res.
+    unfold add_func in Hallocfuncs.
+    inversion Hallocfuncs; subst; clear Hallocfuncs.
+    rewrite map_app app_length /=.
+    rewrite gen_index_extend.
+    specialize (IHmodfuncs ws ws0 (rev l0)).
+    destruct IHmodfuncs as [? [? [? [? ?]]]]; first by rewrite Heqfold_res.
+    repeat split => //; try by eapply IHmodfuncs; rewrite Heqfold_res.
+    + rewrite H.
+      rewrite H0.
+      by rewrite app_length map_length.
+    + rewrite H0.
+      rewrite - app_assoc.
+      f_equal.
+      by rewrite -> list_fmap_app.
+Qed.
+
+Lemma alloc_tab_gen_index modtabtypes ws ws' l:
+  alloc_tabs ws modtabtypes = (ws', l) ->
+  map (fun x => match x with | Mk_tableidx i => i end) l = gen_index (length (s_tables ws)) (length modtabtypes) /\
+  ws'.(s_tables) = ws.(s_tables) ++ fmap (fun '{| tt_limits := {| lim_min := min; lim_max := maxo |} |} => {| table_data := repeat None (ssrnat.nat_of_bin min); table_max_opt := maxo |}) modtabtypes /\
+  ws.(s_funcs) = ws'.(s_funcs) /\
+  ws.(s_mems) = ws'.(s_mems) /\
+  ws.(s_globals) = ws'.(s_globals).
+Proof.
+  unfold alloc_tabs, alloc_Xs.
+  generalize dependent l.
+  generalize dependent ws'.
+  generalize dependent ws.
+  induction modtabtypes using List.rev_ind; move => ws ws' l Halloc.
+  - inversion Halloc; subst; clear Halloc.
+    repeat split => //.
+    simpl.
+    by rewrite app_nil_r.
+  - rewrite fold_left_app in Halloc.
+    remember (fold_left _ modtabtypes (ws,[])) as fold_res.
+    simpl in Halloc.
+    destruct fold_res as [ws0 l0].
+    symmetry in Heqfold_res.
+    unfold alloc_tab, add_table in Halloc.
+    destruct x => /=.
+    destruct tt_limits => /=.
+    specialize (IHmodtabtypes ws ws0 (rev l0)).
+    rewrite Heqfold_res in IHmodtabtypes.
+    inversion Halloc; subst; clear Halloc.
+    simpl in *.
+    rewrite map_app app_length /=.
+    rewrite gen_index_extend.
+    destruct IHmodtabtypes as [? [? [? [? ?]]]] => //.
+    repeat split => //.
+    + rewrite H.
+      rewrite H0.
+      by rewrite app_length map_length.
+    + rewrite H0.
+      rewrite - app_assoc.
+      f_equal.
+      by rewrite -> list_fmap_app => /=.
+Qed.
+
+Lemma alloc_mem_gen_index modmemtypes ws ws' l:
+  alloc_mems ws modmemtypes = (ws', l) ->
+  map (fun x => match x with | Mk_memidx i => i end) l = gen_index (length (s_mems ws)) (length modmemtypes) /\
+  ws'.(s_mems) = ws.(s_mems) ++ fmap (fun '{| lim_min := min; lim_max := maxo |} => {| mem_data := memory_list.mem_make #00%byte (page_size * min)%N; mem_max_opt := maxo |}) modmemtypes /\
+  ws.(s_funcs) = ws'.(s_funcs) /\
+  ws.(s_tables) = ws'.(s_tables) /\
+  ws.(s_globals) = ws'.(s_globals).
+Proof.
+  unfold alloc_mems, alloc_Xs.
+  generalize dependent l.
+  generalize dependent ws'.
+  generalize dependent ws.
+  induction modmemtypes using List.rev_ind; move => ws ws' l Halloc.
+  - inversion Halloc; subst; clear Halloc.
+    repeat split => //=.
+    by rewrite app_nil_r.
+  - rewrite fold_left_app in Halloc.
+    remember (fold_left _ modmemtypes (ws,[])) as fold_res.
+    simpl in Halloc.
+    destruct fold_res as [ws0 l0].
+    symmetry in Heqfold_res.
+    unfold alloc_mem, add_mem in Halloc.
+    destruct x => /=.
+    specialize (IHmodmemtypes ws ws0 (rev l0)).
+    rewrite Heqfold_res in IHmodmemtypes.
+    inversion Halloc; subst; clear Halloc.
+    simpl in *.
+    rewrite map_app app_length /=.
+    rewrite gen_index_extend.
+    destruct IHmodmemtypes as [? [? [? [? ?]]]] => //.
+    repeat split => //.
+    + rewrite H.
+      rewrite H0.
+      by rewrite app_length fmap_length.
+    + rewrite H0.
+      rewrite - app_assoc.
+      f_equal.
+      by rewrite -> list_fmap_app => /=.
+Qed.
+
+Lemma alloc_glob_gen_index modglobs ws g_inits ws' l:
+  length g_inits = length modglobs ->
+  alloc_globs ws modglobs g_inits = (ws', l) ->
+  map (fun x => match x with | Mk_globalidx i => i end) l = gen_index (length (s_globals ws)) (length modglobs) /\
+  ws'.(s_globals) = ws.(s_globals) ++ fmap (fun '({| modglob_type := gt; modglob_init := ge |}, v) => {| g_mut := gt.(tg_mut); g_val := v |} ) (combine modglobs g_inits) /\
+ (* length ws'.(s_globals) = length ws.(s_globals) + length modglobs /\*)
+  ws.(s_funcs) = ws'.(s_funcs) /\
+  ws.(s_tables) = ws'.(s_tables) /\
+  ws.(s_mems) = ws'.(s_mems).
+Proof.
+  unfold alloc_globs, alloc_Xs.
+  generalize dependent l.
+  generalize dependent ws'.
+  generalize dependent ws.
+  generalize dependent g_inits.
+  induction modglobs using List.rev_ind; move => g_inits ws ws' l Hlen Halloc.
+  - inversion Halloc; subst; clear Halloc.
+    repeat split => //=.
+    by rewrite app_nil_r.
+  - destruct g_inits using List.rev_ind; first by destruct modglobs => /=.
+    repeat rewrite app_length in Hlen; simpl in Hlen.
+    repeat rewrite - cat_app in Halloc.
+    rewrite combine_app in Halloc; last by lias.
+    simpl in Halloc.
+    rewrite fold_left_app in Halloc.
+    lazymatch goal with
+    | _: context C [fold_left ?f (combine modglobs g_inits) (ws, [])] |- _ =>
+      remember (fold_left f (combine modglobs g_inits) (ws, [])) as fold_res
+    end.
+    (* rewrite - Heqfold_res in Halloc. *)
+    destruct fold_res as [ws0 l0].
+    symmetry in Heqfold_res.
+    unfold alloc_glob, add_glob in Halloc.
+    simpl in Halloc.
+    inversion Halloc; subst; clear Halloc.
+    rewrite map_app app_length /=.
+    rewrite gen_index_extend.
+    specialize (IHmodglobs g_inits ws ws0 (rev l0)).
+    destruct IHmodglobs as [? [? [? [? ?]]]] => //.
+    + by lias.
+    + by rewrite Heqfold_res.
+    repeat split => //.
+    + rewrite H.
+      rewrite H0.
+      rewrite app_length fmap_length combine_length.
+      repeat f_equal.
+      by lias.
+    + rewrite H0.
+      rewrite - app_assoc.
+      f_equal.
+      rewrite combine_app => /=.
+      rewrite -> list_fmap_app => /=.
+      repeat f_equal.
+      destruct x => //.
+      by lias.
+Qed.
+
+Lemma init_tabs_preserve ws inst e_inits melem ws':
+  init_tabs ws inst e_inits melem = ws' ->
+  ws.(s_funcs) = ws'.(s_funcs) /\
+  ws.(s_mems) = ws'.(s_mems) /\
+  ws.(s_globals) = ws'.(s_globals).
+Proof.
+  move => Hinit.
+  unfold init_tabs in Hinit.
+  rewrite - Hinit.
+  apply fold_left_preserve => //.
+  move => x [n me] Heq.
+  destruct ws, x.
+  simpl in *.
+  destruct Heq as [-> [-> ->]].
+  unfold init_tab => /=.
+  by destruct (nth _ _) eqn:Hl => /=.
+Qed.
+
+Lemma init_mems_preserve ws inst d_inits mdata ws':
+  init_mems ws inst d_inits mdata = ws' ->
+  ws.(s_funcs) = ws'.(s_funcs) /\
+  ws.(s_tables) = ws'.(s_tables) /\
+  ws.(s_globals) = ws'.(s_globals).
+Proof.
+  move => Hinit.
+  unfold init_mems in Hinit.
+  rewrite - Hinit.
+  apply fold_left_preserve => //.
+  move => x [n md] Heq.
+  destruct ws, x.
+  simpl in *.
+  destruct Heq as [-> [-> ->]].
+  by unfold init_mem => /=.
+Qed.
+
+Lemma mod_imps_len_t m t_imps t_exps:
+  module_typing m t_imps t_exps ->
+  get_import_func_count m = length (ext_t_funcs t_imps) /\
+  get_import_table_count m = length (ext_t_tabs t_imps) /\
+  get_import_mem_count m = length (ext_t_mems t_imps) /\
+  get_import_global_count m = length (ext_t_globs t_imps).
+Proof.
+  unfold get_import_func_count, get_import_table_count, get_import_mem_count, get_import_global_count.
+  unfold module_typing.
+  move => Hmt.
+  destruct m.
+  destruct Hmt as [fts [gts [? [? [? [? [? [? [? [Himptype ?]]]]]]]]]].
+  simpl in *.
+  clear - mod_imports Himptype.
+  move : Himptype.
+  move : t_imps fts gts.
+  induction mod_imports; move => t_imps fts gts Himptype => //=.
+  - apply Forall2_nil_inv_l in Himptype as ->.
+    by simpl.
+  - destruct t_imps; first by apply Forall2_nil_inv_r in Himptype.
+    simpl in *.
+    inversion Himptype; subst; clear Himptype.
+    unfold module_import_typing in H2.
+    destruct a, imp_desc => /=; simpl in H2; destruct e => //.
+    all:
+      try by (move/andP in H2;
+      destruct H2 as [Hlen Hnth];
+      move/eqP in Hnth; subst;
+      simpl;
+      apply IHmod_imports in H4 as [? [? [? ?]]] => //;
+      repeat split => //;
+      f_equal).
+    move/eqP in H2; subst.
+    simpl.
+    apply IHmod_imports in H4 as [? [? [? ?]]] => //.
+    repeat split => //.
+    by f_equal.
+Qed.
+
+End Instantiation_properties.
+
